More on trans

src/Lambda.v
@@ -34,26 +34,70 @@ Lemma frob_eq {A}: forall (x: Computation A), x = frob x.
 Proof. destruct x; reflexivity. Qed.
 
 CoInductive bisim {A} : Computation A -> Computation A -> Prop :=
-| BisimRtrn : forall x, bisim (Return x) (Return x)
-| BisimBind : forall (B: Type) (f: B -> Computation A) x, bisim (Bind x f) (Bind x f)
-| BisimStep : forall x y, bisim x y -> bisim (Step x) (Step y)
+| BisimRtrn   : forall x, bisim (Return x) (Return x)
+| BisimBind  : forall (B: Type) (f: B -> Computation A) x, bisim (Bind x f) (Bind x f)
 | BisimStepL : forall x y, bisim x y -> bisim (Step x) y
-| BisimStepR : forall x y, bisim x y -> bisim x (Step y)
+| BisimStepR : forall x y, bisim x y -> bisim  x (Step y)
 | BisimFail: bisim Fail Fail.
+Hint Resolve BisimRtrn : core.
+(*Hint Resolve BisimBind : core.
+Hint Resolve BisimStep : core.
+Hint Resolve BisimStepL : core.
+Hint Resolve BisimStepR : core.
+Hint Resolve BisimFail : core.*)
 
-Theorem bisim_refl {A}: forall (a: Computation A), bisim a a.
-Proof. cofix CIH. intros. destruct a; constructor.
-- apply CIH. Qed.
 
+
+
+(*Theorem bisim_refl {A}: forall (a: Computation A), bisim a a.
+Proof. cofix CIH.  intros. destruct a; constructor; constructor; apply CIH. Qed.
+Hint Resolve bisim_refl : core.
 Theorem bisim_symm {A}: forall (a b: Computation A), bisim a b -> bisim b a.
-Proof. cofix CIH. intros. inversion H; subst; constructor. inversion H; 
+Proof. cofix CIH. intros. inversion H; subst; constructor.
+-  inversion H; 
 repeat (apply CIH in H0; assumption;
   apply CIH in H0; assumption).
 apply CIH in H0; assumption. apply CIH in H0; assumption. Qed.
-
+Hint Resolve bisim_symm : core.*)
 
 Theorem bisim_trans {A}: forall (a b c: Computation A), bisim a b -> bisim b c -> bisim a c.
-Proof. Admitted.
+Proof. cofix CIH. intros. inversion H. subst. inversion H0; subst.
+- auto. 
+- 
+-     as []. inversion H0. inversion H H0; subst; inversion H0; subst.
+- auto. 
+- inversion H; subst.s
+- inversion H; subst. auto. 
+- 
+
+
+
+ inversion H. subst. inversion H0. destruct H0. 
+- auto.
+- constructor. apply CIH with (b:=  y); auto. 
+- constructor. apply CIH with (b:=  y); auto.
+- inversion H. H0. 
+-  destruct H0.
+
+- constructor.  apply bisim_refl.
+- apply bisim_refl.
+- constructor; assumption.
+- constructor; assumption.
+- constructor; assumption.
+- constructor.
+- assumption.
+- constructor. apply BisimStepR in H. apply CIH with (b:= Step y); assumption.
+- constructor. apply CIH with (b:= y); assumption.  
+(*- rewrite (frob_eq x) in *. rewrite (frob_eq c) in *. apply CIH with (b:= Step y). *)
+-  destruct c. destruct x. constructor. inversion H0. subst.
+
+inversion H0. subst. apply  apply CIH with (a:=x) in H0. assumption.  destruct c; destruct x. apply BisimStepR in H. apply CIH with (b:= Step y); assumption. Guarded.
++ 
+ destruct H0. 
+* inversion H0.
+
+rewrite (frob_eq x) in *. apply BisimStepR in H. apply CIH with (b:= Step y); assumption. 
+- assumption. Qed.
 
 Definition const :=nat. 
 
